

1.  $\{f_n\}$  is a sequence of functions on  $[0, 1]$  defined by

$$f_n(x) = \begin{cases} 1 & \text{if } x \in [0, \frac{1}{n}] \\ 0 & \text{if } x \in (\frac{1}{n}, 1] \end{cases}$$

Find  $\lim_{n \rightarrow \infty} \int_0^1 f_n(x) dx$ .

2. Let  $f: [0, 1] \rightarrow \mathbb{R}$  be a function defined by

$$f(x) = \begin{cases} x & \text{if } x \in [0, \frac{1}{2}] \\ 2x - 1 & \text{if } x \in (\frac{1}{2}, 1] \end{cases}$$

$$f(x) = \begin{cases} x & \text{if } x \in [0, \frac{1}{2}] \\ 2x - 1 & \text{if } x \in (\frac{1}{2}, 1] \end{cases} \quad (1)$$

Find  $\int_0^1 f(x) dx$  and  $\int_0^1 f^2(x) dx$ .

3. Let  $f: [0, 1] \rightarrow \mathbb{R}$  be a function defined by  $f(x) = \begin{cases} x & \text{if } x \in [0, \frac{1}{2}] \\ 2x - 1 & \text{if } x \in (\frac{1}{2}, 1] \end{cases}$ . Find  $\int_0^1 f(x) dx$  and  $\int_0^1 f^2(x) dx$ .

4. Let  $f: [0, 1] \rightarrow \mathbb{R}$  be a function defined by  $f(x) = \begin{cases} x & \text{if } x \in [0, \frac{1}{2}] \\ 2x - 1 & \text{if } x \in (\frac{1}{2}, 1] \end{cases}$ . Find  $\int_0^1 f(x) dx$  and  $\int_0^1 f^2(x) dx$ .

$$\begin{aligned} f(x) &= \begin{cases} x & \text{if } x \in [0, \frac{1}{2}] \\ 2x - 1 & \text{if } x \in (\frac{1}{2}, 1] \end{cases} \\ &= \begin{cases} x & \text{if } x \in [0, \frac{1}{2}] \\ 2x - 1 & \text{if } x \in (\frac{1}{2}, 1] \end{cases} \\ &= \begin{cases} x & \text{if } x \in [0, \frac{1}{2}] \\ 2x - 1 & \text{if } x \in (\frac{1}{2}, 1] \end{cases} \end{aligned} \quad (2)$$

Find  $\int_0^1 f(x) dx$  and  $\int_0^1 f^2(x) dx$ .

5. Let  $f: [0, 1] \rightarrow \mathbb{R}$  be a function defined by  $f(x) = \begin{cases} x & \text{if } x \in [0, \frac{1}{2}] \\ 2x - 1 & \text{if } x \in (\frac{1}{2}, 1] \end{cases}$ .

$$f(x) = \begin{cases} x & \text{if } x \in [0, \frac{1}{2}] \\ 2x - 1 & \text{if } x \in (\frac{1}{2}, 1] \end{cases} \quad (3)$$

Find  $\int_0^1 f(x) dx$  and  $\int_0^1 f^2(x) dx$ .

6. Let  $f: [0, 1] \rightarrow \mathbb{R}$  be a function defined by  $f(x) = \begin{cases} x & \text{if } x \in [0, \frac{1}{2}] \\ 2x - 1 & \text{if } x \in (\frac{1}{2}, 1] \end{cases}$ . Find  $\int_0^1 f(x) dx$  and  $\int_0^1 f^2(x) dx$ .

7. Let  $f: [0, 1] \rightarrow \mathbb{R}$  be a function defined by  $f(x) = \begin{cases} x & \text{if } x \in [0, \frac{1}{2}] \\ 2x - 1 & \text{if } x \in (\frac{1}{2}, 1] \end{cases}$ .

የሰነድ ቁጥር	የሰነድ ስም	ቀን
1/7/11	የሰነድ ስም	11/11
2/7/11	የሰነድ ስም	11/11/11
3/7/11	የሰነድ ስም	11/11
4/7/11	የሰነድ ስም	11/11/11

የሰነድ ስም

የሰነድ ስም

$$f(x) = \frac{1}{x} \ln \left( \frac{x+1}{x-1} \right) = \frac{1}{x} \ln \left( \frac{x+1}{x-1} \right) = \frac{1}{x} \ln \left( \frac{x+1}{x-1} \right) = \frac{1}{x} \ln \left( \frac{x+1}{x-1} \right) \quad (1)$$

የሰነድ ስም

የሰነድ ስም

$$f(x) = \frac{1}{x} \ln \left( \frac{x+1}{x-1} \right) \quad (2)$$

የሰነድ ስም

የሰነድ ስም

$$f(x) = \frac{1}{x} \ln \left( \frac{x+1}{x-1} \right) = \frac{1}{x} \ln \left( \frac{x+1}{x-1} \right) = \frac{1}{x} \ln \left( \frac{x+1}{x-1} \right) = \frac{1}{x} \ln \left( \frac{x+1}{x-1} \right) \quad (3)$$

የሰነድ ስም

$$f(x) = \frac{1}{x} \ln \left( \frac{x+1}{x-1} \right) = \frac{1}{x} \ln \left( \frac{x+1}{x-1} \right) = \frac{1}{x} \ln \left( \frac{x+1}{x-1} \right) = \frac{1}{x} \ln \left( \frac{x+1}{x-1} \right) \quad (4)$$

የሰነድ ስም

$$f(x) = \frac{1}{x} \ln \left( \frac{x+1}{x-1} \right) = \frac{1}{x} \ln \left( \frac{x+1}{x-1} \right) = \frac{1}{x} \ln \left( \frac{x+1}{x-1} \right) = \frac{1}{x} \ln \left( \frac{x+1}{x-1} \right) \quad (5)$$

የሰነድ ስም

የሰነድ ስም

የሰነድ ስም

የሰነድ ስም

1. 证明：若  $f(x)$  在  $[a, b]$  上连续，且  $f(a) = f(b)$ ，则存在  $\xi \in (a, b)$ ，使得  $f'(\xi) = 0$ 。

$$f'(x) = \lim_{h \rightarrow 0} \frac{f(x+h) - f(x)}{h} = 0 \quad (1)$$

2. 证明：若  $f(x)$  在  $[a, b]$  上连续，且  $f(a) \neq f(b)$ ，则存在  $\xi \in (a, b)$ ，使得  $f'(\xi) = \frac{f(b) - f(a)}{b - a}$ 。

$$f'(x) = \lim_{h \rightarrow 0} \frac{f(x+h) - f(x)}{h} = \frac{f(b) - f(a)}{b - a} \quad (2)$$

3. 证明：若  $f(x)$  在  $[a, b]$  上连续，且  $f(a) = f(b)$ ，则存在  $\xi \in (a, b)$ ，使得  $f'(\xi) = 0$ 。

4. 证明：若  $f(x)$  在  $[a, b]$  上连续，且  $f(a) \neq f(b)$ ，则存在  $\xi \in (a, b)$ ，使得  $f'(\xi) = \frac{f(b) - f(a)}{b - a}$ 。

5. 证明：若  $f(x)$  在  $[a, b]$  上连续，且  $f(a) = f(b)$ ，则存在  $\xi \in (a, b)$ ，使得  $f'(\xi) = 0$ 。

6. 证明：若  $f(x)$  在  $[a, b]$  上连续，且  $f(a) \neq f(b)$ ，则存在  $\xi \in (a, b)$ ，使得  $f'(\xi) = \frac{f(b) - f(a)}{b - a}$ 。